src/tls/PNE.fsti
@@ -39,7 +39,7 @@ noeq type pn_pkg =
     as_bytes: (i:I.id -> l:pnlen -> pn i l -> GTot (lbytes l)) ->
     repr: (i:I.id{~(safePNE i)} -> l:pnlen -> n:pn i l -> Tot (b:lbytes l{b == as_bytes i l n})) ->
     from_bytes: (i:I.id -> l:pnlen -> b:lbytes l -> GTot (n:pn i l{as_bytes i l n == b})) ->
-    abs: (i:I.id{~(safePNE i)} -> l:pnlen -> b:lbytes l -> Tot (n:pn i l{n == from_bytes i l b})) ->
+    abs: (i:I.id -> l:pnlen -> b:lbytes l -> Tot (n:pn i l{n == from_bytes i l b})) ->
     pn_pkg
 
 let info = pn_pkg
@@ -63,7 +63,17 @@ val pne_state : i:I.id -> u:info -> Type0
 val table : (#i:I.id) -> (#u:info) -> (st:pne_state i u) -> (h:mem) -> GTot (Seq.seq (entry i u))
 
 val footprint : #i:I.id -> #u:info -> st:pne_state i u -> GTot (subrgn table_region)
- 
+
+val frame_table: #i:I.id -> #u:info -> st:pne_state i u -> l:Seq.seq (entry i u) ->
+  h0:mem -> s:Set.set rid -> h1:mem ->
+  Lemma
+    (requires
+      safePNE i /\
+      table st h0 == l /\
+      modifies s h0 h1 /\
+      Set.disjoint s (Set.singleton (footprint st)))
+    (ensures table st h1 == l)
+
 let sample_filter (i:I.id) (u:info) (s:ciphersample) (e:entry i u) : bool =
   Entry?.s e = s
 
@@ -74,6 +84,23 @@ let entry_for_sample (#i:I.id) (#u:info) (s:ciphersample) (st:pne_state i u) (h:
 let fresh_sample (#i:I.id) (#u:info) (s:ciphersample) (st:pne_state i u) (h:mem) :
   GTot bool =
   None? (entry_for_sample s st h)
+
+let find_sample (#i:I.id) (#u:info) (s:ciphersample) (st:pne_state i u) (h:mem) :
+  GTot bool =
+  Some? (entry_for_sample s st h)
+
+
+let sample_epn_filter (i:I.id) (u:info) (s:ciphersample) (#l:pnlen) (ne:epn l) (e:entry i u) : bool =
+  Entry?.s e = s && Entry?.l e = l && Entry?.ne e = ne
+
+let entry_for_sample_epn (#i:I.id) (#u:info) (s:ciphersample) (#l:pnlen) (ne:epn l) (st:pne_state i u) (h:mem) :
+  GTot (option (entry i u)) =
+  Seq.find_l (sample_epn_filter i u s #l ne) (table st h)
+  
+let find_sample_epn (#i:I.id) (#u:info) (s:ciphersample) (#l:pnlen) (ne:epn l) (st:pne_state i u) (h:mem) :
+  GTot bool =
+  Some? (entry_for_sample_epn s ne st h)
+
 
 let sample_cipher (c:cipher) : s:ciphersample =
   Bytes.slice c 0ul 16ul
@@ -90,35 +117,30 @@ val encrypt :
   (st:pne_state i u) ->
   (#l:pnlen) ->
   (n:pn i u l) ->
-  (c:cipher) ->
+  (s:ciphersample) ->
   ST (epn l)
   (requires fun h0 ->
-    fresh_sample (sample_cipher c) st h0)
+    fresh_sample s st h0)
   (ensures fun h0 ne h1 ->
     modifies_one (footprint st) h0 h1 /\
-    (let s = sample_cipher c in
-    table st h1 == Seq.snoc (table st h0) (Entry s ne n)))
+    (safePNE i ==> table st h1 == Seq.snoc (table st h0) (Entry s ne n)))
 
+#reset-options "--z3rlimit 50"
 val decrypt :
   (#i:I.id) ->
   (#u: info) ->
   (st:pne_state i u) ->
   (#l:pnlen) ->
   (ne:epn l) ->
-  (c:cipher) ->
-  ST (option (pn i u l))
+  (s:ciphersample) ->
+  ST (pn i u l)
   (requires fun h0 -> True)
-  (ensures fun h0 on h1 ->
+  (ensures fun h0 n h1 ->
     modifies_none h0 h1 /\
-    (let s = sample_cipher c in
-      (safePNE i ==>
-        (match entry_for_sample s st h0 with
-          | None -> None? on
-          | Some (Entry _ ne' n) -> 
-            if ne = ne' then on = Some n
-            else None? on)
-      )
+    ((safePNE i /\ find_sample s st h0) ==>
+     (match entry_for_sample s st h0 with
+        | Some (Entry _ #l' ne' n') -> (l = l' /\ n = n') <==> (l = l' /\ ne = ne'))
     )
   )
-  
+
 
