src/tls/QUICStream2.fsti
@@ -1,4 +1,4 @@
-module QUICStream
+module QUICStream2
 module HS = FStar.HyperStack 
 
 module I = Crypto.Indexing
@@ -14,15 +14,13 @@ open Mem
 open Pkg
 
 
-let safeId (i:I.id) = AEAD.safeId i
-let safePNE (j:I.id) = PNE.safePNE j
-
 type plainLen = l:nat{l + v AEAD.taglen <= pow2 32 - 1 /\ l + v AEAD.taglen >= 16}
 
-type cipher (i:I.id) (l:plainLen) = lbytes (l + v AEAD.taglen)
+type safeid = i:I.id{Flag.safeId i}
 
-let max_ctr = pow2 62 - 1
+let safeId (i:I.id) = AEAD.safeId i
 
+let safePNE (j:I.id) = PNE.safePNE j
 
 (* plain pkg *)
 val plain: i:I.id -> l:plainLen -> t:Type0{hasEq t}
@@ -35,19 +33,23 @@ val plain_repr : i:I.id{~(AEAD.safeId i)} -> l:plainLen -> p:plain i l -> b:lbyt
 
 let aead_plain_pkg = AEAD.PlainPkg 0 plain plain_as_bytes plain_repr
 
-
 (* nonce pkg *)
 let pnlen = n:nat{n=1 \/ n=2 \/ n=4}
 
-val nonce (i:I.id) (nl:pnlen) : (t:Type0{hasEq t})
+val nonce (i:I.id) (nl:pnlen) : (t:Type0{hasEq t}) //= AEAD.iv (I.cipherAlg_of_id i)
 
-val nonce_as_bytes (i:I.id) (nl:pnlen) (n:nonce i nl) : GTot (AEAD.iv (I.cipherAlg_of_id i))
+val nonce_as_bytes (i:I.id) (nl:pnlen) (n:nonce i nl) : GTot (AEAD.iv (I.cipherAlg_of_id i)) //= n
 
 val nonce_repr (i:I.id{~(safeId i)}) (nl:pnlen) (n:nonce i nl) :
-  Tot (b:AEAD.iv (I.cipherAlg_of_id i){b == nonce_as_bytes i nl n})
+  Tot (b:AEAD.iv (I.cipherAlg_of_id i){b == nonce_as_bytes i nl n}) //= n
 
 let aead_nonce_pkg =
   AEAD.NoncePkg pnlen nonce nonce_as_bytes nonce_repr
+
+
+type cipher (i:I.id) (l:plainLen) = lbytes (l + v AEAD.taglen)
+
+let max_ctr = pow2 62 - 1
 
 
 (* pn pkg *)
@@ -63,11 +65,9 @@ val npn_from_bytes : j:I.id -> l:pnlen -> b:lbytes l -> GTot (n:npn j l{npn_as_b
 
 val npn_abs : j:I.id{~(PNE.safePNE j)} -> l:pnlen -> b:lbytes l -> Tot (n:npn j l{n == npn_from_bytes j l b})
   
-let npn_pkg = PNE.PNPkg npn npn_as_bytes npn_repr npn_from_bytes npn_abs
+//let npn_pkg = PNE.PNPkg npn npn_as_bytes npn_repr npn_from_bytes npn_abs
 
-
-
-let epn = PNE.epn
+type epn (l:pnlen) = lbytes l
 
 type rpn = n:U64.t{U64.v n <= max_ctr}
 
@@ -78,6 +78,7 @@ let rpn_of_nat (j:nat{j<= max_ctr}) : rpn =
 val npn_encode : (j:I.id) -> (r:rpn) -> (l:pnlen) -> (n:npn j l)
 
 val npn_decode : (#j:I.id) -> (#nl:pnlen) -> (n:npn j nl) -> (expected_pn:rpn) -> rpn
+
 
 val create_nonce : #i:I.id -> #alg:I.cipherAlg{alg == I.cipherAlg_of_id i} ->
   iv: AEAD.iv alg -> nl:pnlen -> r:rpn -> Tot (nonce i nl)
@@ -90,13 +91,15 @@ val writer_aead_state : #i:I.id -> #j:I.id -> w:stream_writer i j ->
   aw:AEAD.aead_writer i
   {(AEAD.wgetinfo aw).AEAD.plain == aead_plain_pkg /\
   (AEAD.wgetinfo aw).AEAD.nonce == aead_nonce_pkg} 
+
 val reader_aead_state : #i:I.id -> #j:I.id -> #w:stream_writer i j -> r:stream_reader w ->
   ar:AEAD.aead_reader (writer_aead_state w)
   {(AEAD.rgetinfo ar).AEAD.plain == aead_plain_pkg /\
   (AEAD.rgetinfo ar).AEAD.nonce == aead_nonce_pkg} 
 
-val writer_pne_state : #i:I.id -> #j:I.id -> w:stream_writer i j -> PNE.pne_state j npn_pkg
-val reader_pne_state : #i:I.id -> #j:I.id -> #w:stream_writer i j -> r:stream_reader w -> PNE.pne_state j npn_pkg
+val writer_pne_state : #i:I.id -> #j:I.id -> w:stream_writer i j -> PNE.pne_state j
+
+val reader_pne_state : #i:I.id -> #j:I.id -> #w:stream_writer i j -> r:stream_reader w -> PNE.pne_state j
 
 val invariant: #i:I.id -> #j:I.id -> w:stream_writer i j -> h:mem ->
   t:Type0{t ==> AEAD.winvariant (writer_aead_state w) h} 
@@ -113,17 +116,39 @@ val reader_iv: #i:I.id -> #j:I.id -> #w:stream_writer i j -> r:stream_reader w -
   iv:AEAD.iv (I.cipherAlg_of_id i){iv = writer_iv w}
 
 val expected_pnT: #i:I.id -> #j:I.id -> #w:stream_writer i j -> r:stream_reader w -> h:mem ->
-  GTot rpn
+  GTot rpn        
+
 val expected_pn: #i:I.id -> #j:I.id -> #w:stream_writer i j -> r:stream_reader w -> ST rpn
   (requires fun h0 -> True)
   (ensures fun h0 c h1 -> h0 == h1 /\
     (c == expected_pnT #i #j #w r h0))
 
+(*let highest_pn_or_zero (#i:I.id) (#j:I.id) (#w:stream_writer i j) (r:stream_reader w) (h:mem) : GTot rpn =
+  match highest_pnT r h with
+    | None -> U64.uint_to_t 0
+    | Some x -> x
+*)
+
+(*let pn_filter (i:I.id) (j:I.id) (ns:Seq.seq rpn) (e:stream_entry i j) : bool =
+  let n = Entry?.pn e in
+  Seq.mem n ns
+
+let epn_filter (i:I.id) (j:I.id) (l:pnlen) (ne:epn l) (e:stream_entry i j) : bool =
+  Entry?.nl e = l && Entry?.ne e = ne
+  
+let seq_filter (#a:Type) (f:a -> bool) (s:Seq.seq a) : Seq.seq a =
+  Seq.seq_of_list #a (List.Tot.filter #a f (Seq.seq_to_list #a s))
+
+let log_filter (#i:safeid) (#j:I.id) (w:stream_writer i j) (h:mem{invariant w h}) (ns:Seq.seq rpn) =
+  seq_filter (pn_filter i j ns) (wlog w h)
+
+val rlog: #i:safeid -> #j:I.id -> #w:stream_writer i j -> r:stream_reader w -> h:mem{invariant w h /\ rinvariant r h} ->
+  GTot (s:Seq.seq (stream_entry i j)
+    {s == log_filter w h (pnlog r h)})
+*)
 
 let wincrementable (#i:I.id) (#j:I.id) (w:stream_writer i j) (h:mem) =
   wctrT w h < max_ctr
-
-
 
 type info' = {
   alg: I.aeadAlg;
@@ -164,7 +189,7 @@ val rframe_invariant: #i:I.id -> #j:I.id -> #w:stream_writer i j -> r:stream_rea
   (ensures rinvariant r h1)
 
 
-val wframe_log: #i:I.id{safeId i} -> #j:I.id -> w:stream_writer i j -> l:Seq.seq (AEAD.entry i (AEAD.wgetinfo (writer_aead_state w))) ->
+val wframe_log: #i:safeid -> #j:I.id -> w:stream_writer i j -> l:Seq.seq (AEAD.entry i (AEAD.wgetinfo (writer_aead_state w))) ->
   h0:mem -> ri:rid -> h1:mem ->
   Lemma
   (requires
@@ -176,7 +201,7 @@ val wframe_log: #i:I.id{safeId i} -> #j:I.id -> w:stream_writer i j -> l:Seq.seq
     ~(Set.mem ri (shared_footprint w)))
   (ensures invariant w h1 ==> AEAD.wlog (writer_aead_state w) h1 == l)
 
-val rframe_log: #i:I.id{safeId i} -> #j:I.id -> #w:stream_writer i j -> r:stream_reader w -> l:Seq.seq (AEAD.entry i (AEAD.rgetinfo (reader_aead_state r))) ->
+val rframe_log: #i:safeid -> #j:I.id -> #w:stream_writer i j -> r:stream_reader w -> l:Seq.seq (AEAD.entry i (AEAD.rgetinfo (reader_aead_state r))) ->
   h0:mem -> ri:rid -> h1:mem ->
   Lemma
   (requires
@@ -189,7 +214,7 @@ val rframe_log: #i:I.id{safeId i} -> #j:I.id -> #w:stream_writer i j -> r:stream
   (ensures invariant w h1 ==> AEAD.rlog (reader_aead_state r) h1 == l)
 
 
-val wframe_pnlog: #i:I.id -> #j:I.id -> w:stream_writer i j -> l:Seq.seq (PNE.entry j npn_pkg) ->
+val wframe_pnlog: #i:I.id -> #j:I.id -> w:stream_writer i j -> l:Seq.seq (PNE.entry j) ->
   h0:mem -> ri:rid -> h1:mem ->
   Lemma
   (requires
@@ -200,7 +225,7 @@ val wframe_pnlog: #i:I.id -> #j:I.id -> w:stream_writer i j -> l:Seq.seq (PNE.en
     ~(Set.mem ri (shared_footprint w)))
   (ensures PNE.table (writer_pne_state w) h1 == l)
 
-val rframe_pnlog: #i:I.id -> #j:I.id -> #w:stream_writer i j -> r:stream_reader w -> l:Seq.seq (PNE.entry j npn_pkg) ->
+val rframe_pnlog: #i:I.id -> #j:I.id -> #w:stream_writer i j -> r:stream_reader w -> l:Seq.seq (PNE.entry j) ->
   h0:mem -> ri:rid -> h1:mem ->
   Lemma
   (requires
@@ -218,6 +243,7 @@ val create: i:I.id -> j:I.id -> u:info i j ->
     disjoint u.shared u.local)
   (ensures fun h0 w h1 ->
     invariant w h1 /\
+//    footprint w == Set.union (Set.singleton u.local) (Set.singleton u.parent) /\
     shared_footprint w == Set.singleton u.shared /\
     modifies_none h0 h1 /\
     (Flag.safeId i /\ Flag.safePNE j) ==>
@@ -245,19 +271,44 @@ val createReader: parent:rgn -> #i:I.id -> #j:I.id -> w:stream_writer i j ->
     rinvariant r h1 /\
     modifies_none h0 h1 /\
     (Flag.safeId i /\ Flag.safePNE j) ==>
+//      (AEAD.rlog (reader_aead_state r) h1 == Seq.empty /\
+ //     PNE.table (reader_pne_state r) h1 == Seq.empty /\
       expected_pnT r h1 == U64.uint_to_t 0)
+  //)
+
+
+
+//val rincrementable: #i:I.id -> #w:stream_writer i -> r:stream_reader w -> h:mem -> Type0
+
+
+
+val encrypt_pn
+  (#i:I.id)
+  (#j:I.id)
+  (w:stream_writer i j)
+  (#l:plainLen)
+  (c:cipher i l)
+  (nl:pnlen)
+  ST (epn nl)
+  (requires fun h0 -> wincrementable w h0 /\ invariant w h0)
+  (ensures fun h0 ne h1 ->
+  
+  
+    
 
 
 val encrypt
   (#i:I.id)
   (#j:I.id)
   (w:stream_writer i j)
+//  (ad:AEAD.adata)
   (nl:pnlen)
   (l:plainLen)
   (p:plain i l):
   ST ((epn nl) * (cipher i l))
   (requires fun h0 -> wincrementable w h0 /\ invariant w h0)
-  (ensures fun h0 (ne,c) h1 ->
+  (ensures fun h0 res h1 ->
+    let ((ne:epn nl),(c:cipher i l)) = res in
     let aw = writer_aead_state w in
     let ps = writer_pne_state w in
     invariant w h1 /\
@@ -266,13 +317,21 @@ val encrypt
       let rpn = rpn_of_nat (wctrT w h0) in
       let npn = npn_encode j rpn nl in
       let s = PNE.sample_cipher c in
-      let alg = I.cipherAlg_of_aeadAlg ((AEAD.wgetinfo aw).AEAD.alg) in
-      let n = create_nonce #i #alg (writer_iv w) nl rpn in
+      let alg' = I.cipherAlg_of_aeadAlg ((AEAD.wgetinfo aw).AEAD.alg) in
+      let n = create_nonce #i #alg' (writer_iv w) nl rpn in
       let ad = Bytes.empty_bytes in
       AEAD.wlog aw h1 == Seq.snoc (AEAD.wlog aw h0) (AEAD.Entry #i #(AEAD.wgetinfo aw) #nl n ad p c) /\
-      PNE.table ps h1 == Seq.snoc (PNE.table ps h0) (PNE.Entry #j #npn_pkg s #nl ne npn))) /\
+      PNE.table ps h1 == Seq.snoc (PNE.table ps h0) (PNE.Entry #j s ))) /\
     modifies (Set.union (footprint w) (shared_footprint w)) h0 h1)
 
+
+//val adata_of_entry: #i:I.id -> stream_entry i -> GTot AEAD.adata
+
+//val cipher_of_entry: #i:I.id -> stream_entry i -> GTot //(lmax:AEAD.plainLen & c:cipher i lmax)
+
+//let matches (#i:I.id) (e:stream_entry i) (ad:AEAD.adata) (lmax:AEAD.plainLen) (c:cipher i lmax) : GTot bool =
+//  let (|lmax', c'|) = cipher_of_entry e in
+ //   adata_of_entry e = ad && lmax' = lmax && c' = c
 
 
 #reset-options "--z3rlimit 50"
@@ -282,6 +341,7 @@ val decrypt
   (#j:I.id)
   (#w:stream_writer i j)
   (r:stream_reader w)
+//  (ad:AEAD.adata)
   (#nl:pnlen)
   (ne:epn nl)
   (l:plainLen)
@@ -297,22 +357,24 @@ val decrypt
     (None? res ==> expected_pnT r h1 == expected_pnT r h0) /\    
     ((Flag.safePNE j /\ Flag.safeId i) ==> 
       (let s = PNE.sample_cipher c in
-      match PNE.entry_for_sample_epn s ne ps h0 with
+      match PNE.entry_for_sample s ps h0 with
         | None -> None? res
-        | Some (PNE.Entry  _ _ npn) ->
-	  let rpn = npn_decode #j #nl npn (expected_pnT r h0) in
-          let alg = I.cipherAlg_of_aeadAlg ((AEAD.rgetinfo ar).AEAD.alg) in
-          let n = create_nonce #i #alg (reader_iv r) nl rpn in
-          match AEAD.wentry_for_nonce aw #nl n h0 with
-	    | None -> None? res
-	    | Some (AEAD.Entry _  ad' #l' p' c')  -> 
-	      if ad' = Bytes.empty_bytes && l' = l && c' = c then 
-	        (res = Some p' /\
+        | Some (PNE.Entry _ #nl' ne' npn) ->
+          if nl = nl' && ne = ne' then
+	    let rpn = npn_decode #j #nl npn (expected_pnT r h0) in
+            let alg' = I.cipherAlg_of_aeadAlg ((AEAD.rgetinfo ar).AEAD.alg) in
+            let n = create_nonce #i #alg' (reader_iv r) nl rpn in
+            match AEAD.wentry_for_nonce aw #nl n h0 with
+	      | None -> None? res
+	      | Some (AEAD.Entry _  ad' #l' p' c')  -> 
+	        if ad' = Bytes.empty_bytes && l' = l && c' = c then 
+	          (res = Some p' /\
                   (if U64.v rpn >= U64.v (expected_pnT r h0) && U64.v rpn < max_ctr then
                     expected_pnT r h1 = rpn_of_nat (U64.v rpn + 1)
                   else
                     expected_pnT r h1 = expected_pnT r h0))                  
 	        else None? res
+	  else None? res
       )
     )
   )
