src/tls/PNE2.fsti
@@ -1,0 +1,110 @@
+module PNE2
+module HS = FStar.HyperStack
+
+module I = Crypto.Indexing
+module U32 = FStar.UInt32
+module U128 = FStar.UInt128
+
+open FStar.HyperStack
+open FStar.Seq
+open FStar.Monotonic.Seq
+open FStar.Error
+open FStar.Bytes
+
+open FStar.Bytes
+open FStar.UInt32
+open Mem
+open Pkg
+
+
+//let pnlen = 4
+
+val table_region : rgn
+
+let safePNE (i:I.id) = Flag.safePNE i
+
+type cipher = b:bytes{Bytes.length b >= 16}
+
+type mask = lbytes 16
+
+type ciphersample = lbytes 16
+
+//type pnlen = n:nat{n<=16}
+//let pnlen = n:nat{n=1 \/ n=2 \/ n=4}
+
+//type epn (l:pnlen) = lbytes l
+
+(*
+noeq type pn_pkg =
+  | PNPkg:
+    pn: (i:I.id -> l:pnlen -> (t:Type0{hasEq t})) ->
+    as_bytes: (i:I.id -> l:pnlen -> pn i l -> GTot (lbytes l)) ->
+    repr: (i:I.id{~(safePNE i)} -> l:pnlen -> n:pn i l -> Tot (b:lbytes l{b == as_bytes i l n})) ->
+    from_bytes: (i:I.id -> l:pnlen -> b:lbytes l -> GTot (n:pn i l{as_bytes i l n == b})) ->
+    abs: (i:I.id{~(safePNE i)} -> l:pnlen -> b:lbytes l -> Tot (n:pn i l{n == from_bytes i l b})) ->
+    pn_pkg
+
+let info = pn_pkg
+
+let pn (i:I.id) (u:info) (l:pnlen) = PNPkg?.pn u i l
+
+let repr (i:I.id{~(safePNE i)}) (u:info) (l:pnlen) (n:pn i u l) = PNPkg?.repr u i l n
+
+let abs (i:I.id{~(safePNE i)}) (u:info) (l:pnlen) (b:lbytes l) = PNPkg?.abs u i l b
+*)
+type entry (i:I.id) =
+  | Entry :
+    s:ciphersample ->
+    m:mask ->
+    entry i
+
+val pne_state : i:I.id -> Type0
+
+val table : (#i:I.id) -> (st:pne_state i) -> (h:mem) -> GTot (Seq.seq (entry i))
+
+val footprint : #i:I.id -> st:pne_state i -> GTot (subrgn table_region)
+
+val frame_table: #i:I.id -> st:pne_state i -> l:Seq.seq (entry i) ->
+  h0:mem -> s:Set.set rid -> h1:mem ->
+  Lemma
+    (requires
+      safePNE i /\
+      table st h0 == l /\
+      modifies s h0 h1 /\
+      Set.disjoint s (Set.singleton (footprint st)))
+    (ensures table st h1 == l)
+
+let sample_filter (i:I.id) (s:ciphersample) (e:entry i) : bool =
+  Entry?.s e = s
+
+let entry_for_sample (#i:I.id) (s:ciphersample) (st:pne_state i) (h:mem) :
+  GTot (option (entry i)) =
+  Seq.find_l (sample_filter i s) (table st h)
+  
+let fresh_sample (#i:I.id) (s:ciphersample) (st:pne_state i) (h:mem) :
+  GTot bool =
+  None? (entry_for_sample s st h)
+
+let sample_cipher (c:cipher) : s:ciphersample =
+  Bytes.slice c 0ul 16ul
+
+val create (i:I.id) : ST (pne_state i)
+  (requires fun _ -> True)
+  (ensures fun h0 st h1 ->
+    modifies_none h0 h1 /\
+    table st h1 == Seq.empty)
+
+val compute :
+  (#i:I.id) ->
+  (st:pne_state i) ->
+  (c:cipher) ->
+  ST (mask)
+  (requires fun h0 -> True)
+//    fresh_sample (sample_cipher c) st h0)
+  (ensures fun h0 m h1 ->
+    let s = sample_cipher c in
+    modifies_one (footprint st) h0 h1 /\
+    (safePNE i ==>
+      (match (entry_for_sample s st h0) with
+        | None -> table st h1 == Seq.snoc (table st h0) (Entry s m)
+        | Some (Entry _ m') -> m = m')))
